Revert "wip new loop"
This reverts commit c0cbcdaad602488a03ed96d9748239b967da39ed.

src/lib/poly/Kuiper.Poly.HReduce.fst
@@ -215,18 +215,6 @@ fn iteration
   }
 }
 
-fn spow2_below (i : ref SZ.t) (b : SZ.t)
-  (#vi : erased sz {reveal vi < 32})
-  preserves i |-> vi
-  returns res : bool
-  ensures
-    pure (res <==> (spow2 vi < b))
-{
-  open FStar.SizeT;
-  let vi = !i;
-  (spow2 vi <^ b);
-}
-
 inline_for_extraction noextract
 fn d_reduce
   (#et:Type0) {| scalar et |}
@@ -255,13 +243,14 @@ fn d_reduce
   (**)if_intro_true (gpu_pts_to_slice_sum a tid (tid + 1) s);
 
   open FStar.SizeT;
-  nuwhile (spow2_below n nth)
-    invariant
-      exists* (it : sz).
+  while (let it = !n; (spow2 it <^ nth))
+    invariant c.
+      exists* (it:sz).
+        gpu **
         pts_to n it **
         mbarrier_tok nth (barrier_matrix nth a s) it tid **
         if_ (div_pow2 (SZ.v it) (SZ.v tid)) (gpu_pts_to_slice_sum a tid (min (tid + pow2 it) nth) s) **
-        pure (it < 32)
+        pure (c == (pow2 it < nth) /\ SZ.v it < 32)
   {
     let it = !n;
     iteration nth a s tid it;
